\noindent Teoremas Booleanos

\begin{enumerate}[(1)]
\item $x.0=0$
\item $x.1=x$
\item $x.x=x$
\item $x.\overline{x}=0$
\item $x+0=x$
\item $x+1=1$
\item $x+x=x$
\item $x+\overline{x}=x$
\item $x+y=y+x$
\item $x.y=y.x$
\item $x+(y+z)=(x+y)+z=x+y+z$
\item $x.(y.z)=(x.y).z=x.y.z$
\item a) $x.(y+z)=xy+xz$  \hfil b) $(w+x).(y+z)=wy+xy+wz+xz$
\item $x+x.y=x$
\item $x+\overline{x}.y=x+y$
\item $\overline{x}+x.y=\overline{x}+y$
\item $\overline{x+y}=\overline{x} . \overline{y}$ \hfill Teorema DeMorgan
\item $\overline{x.y}=\overline{x} + \overline{y}$ \hfill Teorema DeMorgan
\end{enumerate}